theories/iris/memory.v
@@ -238,7 +238,7 @@ Ltac open_rt H :=
   iDestruct H
     as "(%rm & %lm & %hm &
          Haddr & Hroot & Hlayout & Hheap & Hrti & %Hinj & Hownmm &
-         Howngc & %Hrootok & Hrootmem & %Hheapok & Hheapmem)".
+         Howngc & %Hrootok & Hrootmem & %Hlayoutok & %Hheapok & Hheapmem)".
 
 Section Rules.
 
